CellularAutomatas/proofs/rt_eq_2n_iff_rt_eq_rt_rev/x_prefix_advice_two_stage.lean
@@ -1,6 +1,6 @@
 import CellularAutomatas.defs
 import CellularAutomatas.proofs.basic
-import CellularAutomatas.proofs.exp_middle_two_stage
+import CellularAutomatas.proofs.middle_exp_two_stage
 import CellularAutomatas.proofs.finite_state_transducers
 import CellularAutomatas.proofs.rt_eq_2n_iff_rt_eq_rt_rev.nextpow2
 import Mathlib.Data.Nat.Log
